Building the correctness instance for L1g to L2.
Also, removed old, no-longer-needed definitions from certiClasses.v

Randy: certiL1g_to_L2Correct, which
is the last item in L2_typeStripped/instances.v, is the fully
instantiated correctness property for L1g to L2.
The functions L1g.flattenApp and L2.flattenApp need to be defined.
Also, the GoodTerm instances for L1g and L2 need to be strenghtened as needed for the 2 subgoals.
I will let you try to finish the two subgoals.

certicoq/theories/L1g/instances.v
@@ -2,6 +2,8 @@ Require Import L1g.compile.
 Require Import L1g.wcbvEval.
 Require Import certiClasses.
 Require Import Common.Common.
+Require Import Common.classes.
+Require Import certiClasses2.
 
 Instance bigStepOpSemL1gTerm : BigStepOpSem (Program L1g.compile.Term) :=
   BigStepOpWEnv _ WcbvEval.
@@ -10,7 +12,35 @@ Instance bigStepOpSemL1gTerm : BigStepOpSem (Program L1g.compile.Term) :=
 Instance WfL1gTerm : GoodTerm (Program L1g.compile.Term) :=
   fun _  => True.
 
-Instance certiL1g : CerticoqLanguage (Program L1g.compile.Term) := {}.
+Require Import SquiggleEq.UsefulTypes.
+Require Import DecidableClass.
+
+Definition flattenApp (t:L1g.compile.Term) : (L1g.compile.Term * (list L1g.compile.Term)).
+Admitted.
+
+Global Instance QuestionHeadL2Term : QuestionHead (Program L1g.compile.Term) :=
+fun q t =>
+match q, fst (flattenApp (main t)) with
+| Cnstr ind ci, TConstruct ind2 ci2 _(*nargs*) =>
+  andb (decide (ind=ind2)) (decide (ci=ci2))
+| Abs, TLambda _ _ _ => true
+| _, _ => false 
+end.
+
+Global Instance ObsSubtermL2Term : ObserveNthSubterm (Program L1g.compile.Term) :=
+fun n t =>
+match  (flattenApp (main t)) with
+| (TConstruct _ _ _ , subterms) =>
+  match List.nth_error subterms  n with
+  | Some st => Some {| env := env t; main := st |}
+  | None => None
+  end
+| _ => None
+end.
+
+
+
+Instance certiL1g : CerticoqLanguage (Program L1g.compile.Term):= {}.
 
 Local Generalizable Variable Lj.
 
@@ -22,13 +52,15 @@ Definition translateTo `{CerticoqTranslation (Program L1g.compile.Term) Lj}
 
 Arguments translateTo Lj {H} p.
 
-Definition ctranslateTo {Term Value BigStep WF} 
-  (Lj : @CerticoqLanguage Term Value BigStep WF)
+Require Import certiClasses.
+
+Definition ctranslateTo {Term Value BigStep WF QH ObsS } 
+  (Lj : @CerticoqLanguage Term Value BigStep WF QH ObsS)
    `{CerticoqTranslation (Program L1g.compile.Term) (cTerm Lj)}
    : program -> exception (cTerm Lj) :=
   translateTo (cTerm Lj).
 
-Arguments ctranslateTo {Term0} {Value} {BigStep} {WF} Lj {H} p.
+Arguments ctranslateTo {Term0} {Value} {BigStep} {WF} {QH} {ObsS} Lj {H} p.
 
 
 
