certicoq/theories/L2_typeStripped/instances.v
@@ -3,15 +3,48 @@ Require Import L2.wcbvEval.
 Require Import certiClasses.
 Require Import Common.Common.
 Require Import L1g.instances.
+Require Import certiClasses2.
 
 Instance bigStepOpSemL2Term : BigStepOpSem (Program L2.compile.Term) :=
   BigStepOpWEnv _ WcbvEval.
 
-(** FIX!! *)
+(** If the compiler only correctly compiles terms with some properties, add them here. *)
 Instance WfL2Term : GoodTerm (Program L2.compile.Term) :=
   fun _  => True.
 
-Instance certiL2 : CerticoqLanguage (Program L2.compile.Term) := {}.
+
+Require Import SquiggleEq.UsefulTypes.
+Require Import DecidableClass.
+
+Definition flattenApp (t:L2.compile.Term) : (L2.compile.Term * (list L2.compile.Term)).
+Admitted.
+
+Global Instance QuestionHeadL2Term : QuestionHead (Program L2.compile.Term) :=
+fun q t =>
+match q, fst (flattenApp (main t)) with
+| Cnstr ind ci, TConstruct ind2 ci2 _(*nargs*) =>
+  andb (decide (ind=ind2)) (decide (ci=ci2))
+| Abs, TLambda _ _ => true
+| _, _ => false 
+end.
+
+Global Instance ObsSubtermL2Term : ObserveNthSubterm (Program L2.compile.Term) :=
+fun n t =>
+match  (flattenApp (main t)) with
+| (TConstruct _ _ _ , subterms) =>
+  match List.nth_error subterms  n with
+  | Some st => Some {| env := env t; main := st |}
+  | None => None
+  end
+| _ => None
+end.
+
+Global Instance certiL2Eval : BigStepOpSem (Program L2.compile.Term).
+  apply BigStepOpWEnv.
+  apply WcbvEval.
+Defined.
+
+Global Instance certiL2 : CerticoqLanguage (Program L2.compile.Term).
 
 Instance certiL1g_to_L2: 
   CerticoqTotalTranslation (Program L1g.compile.Term)
@@ -21,9 +54,18 @@ Instance certiL1g_to_L2:
 
 Require Import certiClasses2.
 
-Check (@CerticoqTranslationCorrect _ _ bigStepOpSemL2Term WfL2Term).
 
-(***
-Instance certiL1g_to_L2Correct :
-  CerticoqTranslationCorrect bigStepOpSemL2Term WfL2Term.
-***)
+Global Instance certiL1g_to_L2Correct :  CerticoqTranslationCorrect certiL1g certiL2.
+Proof.
+  split.
+  - intros ? ?. simpl. unfold translateT, certiL1g_to_L2.
+    (* The GoodTerm instance of  L1g and L2 may need to be strengthened to complete the next
+      subgoal. Currently, they evaluete to True, which is trivial.
+      unfold goodTerm in *. 
+
+     *) admit.
+  - intros ? ?. 
+    repeat progress (unfold bigStepEval, bigStepEvalSame,
+                     liftBigStepException, bigStepOpSemL1gTerm, translate, translateT, BigStepOpWEnv,
+                     liftTotal, certiL2Eval, certiL1g_to_L2). simpl.
+Admitted.    
